Moved the global state of the Composition Theorem theory to outside the abstract module, so we won't have to have module restrictions for each hybrid game. (Not that UCComposition is now a concrete theory, so it can be `require import`d. The inner abstract theory is cloned for each hybrid game.)

common/UCComposition.ec
@@ -1,6 +1,53 @@
-(* Abstract Theory for Composition Theorem Definitions and Proofs *)
+(* Theory for Composition Theorem Definitions and Proofs *)
 
 require import UCCore UCListAux.
+
+(* global variables of all instances of abstract theory *)
+
+clone MakeInterface as CompEnvMakeInt
+proof *.
+module CompEnvMI = CompEnvMakeInt.MI.
+
+print CompEnvMakeInt.MI.
+
+(* we use the module restriction -CompGlobs for all instances
+   of the Composition abstract theory
+
+   print glob CompGlobs is
+
+     CompGlobs.ce_func : addr
+     CompGlobs.ce_stub_st : msg option
+     CompGlobs.mrfc_self : addr
+     CompEnvMakeInt.MI.func : addr
+     CompEnvMakeInt.MI.in_guard : int fset
+ *)
+
+module CompGlobs = {
+  (* state of instances of MakeRFComp *)
+
+  var mrfc_self : addr
+
+  (* state of instances of CompEnv *)
+
+  var ce_stub_st : msg option
+  var ce_func    : addr
+
+  (* dummy procedure that is only here so that glob CompGlobs
+     includes the global variables of CompEnvMI; this simplifies
+     module restrictions *)
+
+  proc comp_env_make_int_dummy() : unit = {
+    var addr : addr; var in_guard : int fset;
+    addr <- CompEnvMI.func; in_guard <- CompEnvMI.in_guard;
+  }    
+}.
+
+(* abstract theory for composition theorem
+
+   each instance shares the same globals, which simplifies
+   module restrictions *)
+
+abstract theory Composition.
 
 (* begin theory parameters *)
 
@@ -15,10 +62,8 @@ axiom change_pari_valid : 1 <= change_pari <= rf_info.`rfi_num_params.
 (* end theory parameters *)
 
 module MakeRFComp (Rest : FUNC, Par : FUNC) : FUNC = {
-  var self : addr
-
   proc init(_self : addr) : unit = {
-    self <- _self;
+    CompGlobs.mrfc_self <- _self;
     Rest.init(_self);
     Par.init(_self ++ [change_pari]);
   }
@@ -38,18 +83,18 @@ module MakeRFComp (Rest : FUNC, Par : FUNC) : FUNC = {
         not_done <- false; r <- None;
       }
       elif (m.`1 = Dir) {
-        if (m.`3.`1 = self) {
-          if (envport self m.`2) {
+        if (m.`3.`1 = CompGlobs.mrfc_self) {
+          if (envport CompGlobs.mrfc_self m.`2) {
             not_done <- false;
           }
-          elif (! (addr_eq_param rf_info self m.`2.`1 \/
-                   addr_eq_subfun rf_info self m.`2.`1)) {
+          elif (! (addr_eq_param rf_info CompGlobs.mrfc_self m.`2.`1 \/
+                   addr_eq_subfun rf_info CompGlobs.mrfc_self m.`2.`1)) {
             not_done <- false; r <- None;
           }
         }
-        elif (addr_eq_param rf_info self m.`3.`1 \/
-              addr_eq_subfun rf_info self m.`3.`1) {
-          if (m.`2.`1 <> self) {
+        elif (addr_eq_param rf_info CompGlobs.mrfc_self m.`3.`1 \/
+              addr_eq_subfun rf_info CompGlobs.mrfc_self m.`3.`1) {
+          if (m.`2.`1 <> CompGlobs.mrfc_self) {
             not_done <- false; r <- None;
           }
         }
@@ -62,15 +107,15 @@ module MakeRFComp (Rest : FUNC, Par : FUNC) : FUNC = {
         if (m.`2.`1 <> adv) {
           r <- None;
         }
-        elif (m.`3.`1 = self \/
-              addr_eq_subfun rf_info self m.`3.`1) {
+        elif (m.`3.`1 = CompGlobs.mrfc_self \/
+              addr_eq_subfun rf_info CompGlobs.mrfc_self m.`3.`1) {
           if (! rf_info.`rfi_adv_pi_begin < m.`2.`2 <=
                 rf_info.`rfi_adv_pi_main_end) {
             r <- None;
           }
         }
-        elif (addr_ge_param rf_info self m.`3.`1) {
-          pari <- head_of_drop_size_first 0 self m.`3.`1;
+        elif (addr_ge_param rf_info CompGlobs.mrfc_self m.`3.`1) {
+          pari <- head_of_drop_size_first 0 CompGlobs.mrfc_self m.`3.`1;
           if (! (nth1_adv_pi_begin_params rf_info pari <= m.`2.`2 <=
                  nth1_adv_pi_end_params rf_info pari)) {
             r <- None;
@@ -88,7 +133,7 @@ module MakeRFComp (Rest : FUNC, Par : FUNC) : FUNC = {
     var r : msg option <- None;
     var not_done : bool <- true;
     while (not_done) {
-      if (self ++ [change_pari] <= m.`2.`1) {
+      if (CompGlobs.mrfc_self ++ [change_pari] <= m.`2.`1) {
         r <@ Par.invoke(m);
       }
       else {
@@ -101,12 +146,12 @@ module MakeRFComp (Rest : FUNC, Par : FUNC) : FUNC = {
 
   proc invoke(m : msg) : msg option = {
     var r : msg option <- None;
-    (* we can assume m.`3.`1 is not >= self *)
-    if ((m.`1 = Dir /\ m.`2.`1 = self) \/
+    (* we can assume m.`3.`1 is not >= CompGlobs.mrfc_self *)
+    if ((m.`1 = Dir /\ m.`2.`1 = CompGlobs.mrfc_self) \/
         (m.`1 = Adv /\
-         (m.`2.`1 = self \/
-          addr_ge_param rf_info self m.`2.`1 \/
-          addr_eq_subfun rf_info self m.`2.`1))) {
+         (m.`2.`1 = CompGlobs.mrfc_self \/
+          addr_ge_param rf_info CompGlobs.mrfc_self m.`2.`1 \/
+          addr_eq_subfun rf_info CompGlobs.mrfc_self m.`2.`1))) {
       r <@ loop(m);
     }
     return r;
@@ -187,7 +232,7 @@ lemma MakeRFComp_after_par_or_rest_return
   phoare
   [MakeRFComp(Rest, Par).after_par_or_rest :
    r = r' /\
-   after_par_or_rest_return MakeRFComp.self r orig_dest_addr ==>
+   after_par_or_rest_return CompGlobs.mrfc_self r orig_dest_addr ==>
    res.`1 = r' /\ res.`1 = Some res.`2 /\ !res.`3] = 1%r.
 proof.
 proc => /=.
@@ -208,7 +253,7 @@ lemma MakeRFComp_after_par_or_rest_continue
   phoare
   [MakeRFComp(Rest, Par).after_par_or_rest :
    r = r' /\
-   after_par_or_rest_continue MakeRFComp.self r orig_dest_addr ==>
+   after_par_or_rest_continue CompGlobs.mrfc_self r orig_dest_addr ==>
    res.`1 = r' /\ res.`1 = Some res.`2 /\ res.`3] = 1%r.
 proof.
 proc => /=.
@@ -219,7 +264,7 @@ qed.
 lemma MakeRFComp_after_par_or_rest_error (Rest <: FUNC) (Par <: FUNC) :
   phoare
   [MakeRFComp(Rest, Par).after_par_or_rest :
-   after_par_or_rest_error MakeRFComp.self r orig_dest_addr ==>
+   after_par_or_rest_error CompGlobs.mrfc_self r orig_dest_addr ==>
    res.`1 = None /\ ! res.`3] = 1%r.
 proof.
 proc => /=.
@@ -376,34 +421,27 @@ smt(mem_range rfi_valid_lt_par_indices_implies_lt_param_adv_pi_begins).
 smt(mem_range rfi_valid_lt_par_indices_implies_lt_param_adv_pi_begins).
 qed.
 
-clone MakeInterface as MakeInt'
-proof *.
-
-module MI' = MakeInt'.MI.
-
 module CompEnv (Rest : FUNC, Env : ENV, Inter : INTER) = {
-  var stub_st : msg option
-  var func : addr
-
   module StubPar : FUNC = {
     proc init(func : addr) : unit = { }
 
     proc invoke(m : msg) : msg option = {
       var r : msg option;
-      if (stub_st <> None) {
-        r <- stub_st; stub_st <- None;
+      if (CompGlobs.ce_stub_st <> None) {
+        r <- CompGlobs.ce_stub_st; CompGlobs.ce_stub_st <- None;
       }
       else {
         r <@ Inter.invoke(m);
         if (r <> None) {
           m <- oget r;
           if (m.`1 = Adv) {
-            stub_st <- Some m;
+            CompGlobs.ce_stub_st <- Some m;
             (* only mode and destination port matter (destination port id
                must simply be > 0) *)
             r <-
               Some
-              (Adv, (adv, 1), (func ++ [change_pari], 1), TagNoInter, []);
+              (Adv, (adv, 1), (CompGlobs.ce_func ++ [change_pari], 1),
+               TagNoInter, []);
           }
         }
       }
@@ -416,19 +454,20 @@ module CompEnv (Rest : FUNC, Env : ENV, Inter : INTER) = {
 
     proc invoke(m : msg) : msg option = {
       var r : msg option;
-      if (stub_st <> None) {
-        r <- stub_st; stub_st <- None;
+      if (CompGlobs.ce_stub_st <> None) {
+        r <- CompGlobs.ce_stub_st; CompGlobs.ce_stub_st <- None;
       }
       else {
         r <@ Inter.invoke(m);
         if (r <> None) {
           m <- oget r;
           if (m.`1 = Dir) {
-            stub_st <- Some m;
+            CompGlobs.ce_stub_st <- Some m;
             (* only mode and destination address matter *)
             r <-
               Some
-              (Adv, (func ++ [change_pari], 1), (adv, 1), TagNoInter, []);
+              (Adv, (CompGlobs.ce_func ++ [change_pari], 1),
+               (adv, 1), TagNoInter, []);
           }
         }
       }
@@ -440,20 +479,20 @@ module CompEnv (Rest : FUNC, Env : ENV, Inter : INTER) = {
 
   proc main(func_ : addr, in_guard : int fset) : bool = {
     var b : bool;
-    stub_st <- None;
-    func <- take (size func_ - 1) func_;
-    b <@ Exper(MI'(MakeRFComp(Rest, StubPar), StubAdv), Env)
-           .main(func, in_guard `\` rest_adv_pis);
+    CompGlobs.ce_stub_st <- None;
+    CompGlobs.ce_func <- take (size func_ - 1) func_;
+    b <@ Exper(CompEnvMI(MakeRFComp(Rest, StubPar), StubAdv), Env)
+           .main(CompGlobs.ce_func, in_guard `\` rest_adv_pis);
     return b;
   }
 }.
 
 section.
 
-declare module Env  <: ENV{-MI, -CompEnv}.
-declare module Adv  <: ADV{-MI, -CompEnv, -Env}.
-declare module Rest <: FUNC{-MI, -CompEnv, -Env, -Adv}.
-declare module Par  <: FUNC{-MI, -CompEnv, -Env, -Adv, -Rest}.
+declare module Env  <: ENV{-MI, -CompGlobs}.
+declare module Adv  <: ADV{-MI, -CompGlobs, -Env}.
+declare module Rest <: FUNC{-MI, -CompGlobs, -Env, -Adv}.
+declare module Par  <: FUNC{-MI, -CompGlobs, -Env, -Adv, -Rest}.
 
 declare op invar_rest : glob Rest -> bool.
 declare op term_rest  : glob Rest -> int.
@@ -511,15 +550,16 @@ seq 3 3 :
   (={glob Env, glob Adv, glob Rest, glob Par} /\
    invar_rest (glob Rest){1} /\ invar_par (glob Par){1} /\
    _self{1} = func' /\ _self{1} = func{1} /\
-   _self{1} = MI.func{1} /\ _self{1} = MakeRFComp.self{1} /\
+   _self{1} = MI.func{1} /\ _self{1} = CompGlobs.mrfc_self{1} /\
    in_guard{1} = in_guard_low' /\ in_guard{1} = MI.in_guard{1} /\
-   _self{2} = func' /\ _self{2} = func0{2} /\ _self{2} = MI'.func{2} /\
-   _self{2} = MakeRFComp.self{2} /\ _self{2} = CompEnv.func{2} /\
+   _self{2} = func' /\ _self{2} = func0{2} /\
+   _self{2} = CompEnvMI.func{2} /\
+   _self{2} = CompGlobs.mrfc_self{2} /\ _self{2} = CompGlobs.ce_func{2} /\
    MI.func{2} = func' ++ [change_pari] /\
-   in_guard1{2} = MI'.in_guard{2} /\
+   in_guard1{2} = CompEnvMI.in_guard{2} /\
    in_guard1{2} = in_guard_low' /\
    MI.in_guard{2} = in_guard_low' `|` rest_adv_pis /\
-   CompEnv.stub_st{2} = None).
+   CompGlobs.ce_stub_st{2} = None).
 call (_ : true).
 call Par_init.
 call Rest_init.
@@ -531,13 +571,13 @@ call
   (_ :
    ={glob Adv, glob Rest, glob Par} /\
    invar_rest (glob Rest){1} /\ invar_par (glob Par){1} /\
-   MI.func{1} = func' /\ MakeRFComp.self{1} = func' /\
+   MI.func{1} = func' /\ CompGlobs.mrfc_self{1} = func' /\
    MI.in_guard{1} = in_guard_low' /\
-   MI'.func{2} = func' /\ MakeRFComp.self{2} = func' /\
-   CompEnv.func{2} = func' /\ MI.func{2} = func' ++ [change_pari] /\
-   MI'.in_guard{2} = in_guard_low' /\
+   CompEnvMI.func{2} = func' /\ CompGlobs.mrfc_self{2} = func' /\
+   CompGlobs.ce_func{2} = func' /\ MI.func{2} = func' ++ [change_pari] /\
+   CompEnvMI.in_guard{2} = in_guard_low' /\
    MI.in_guard{2} = in_guard_low' `|` rest_adv_pis /\
-   CompEnv.stub_st{2} = None).
+   CompGlobs.ce_stub_st{2} = None).
 proc.
 if => //.
 inline loop.
@@ -550,9 +590,9 @@ qed.
 end section.
 
 lemma compos_bridge
-      (Env <: ENV{-MI, -CompEnv}) (Adv <: ADV{-MI, -CompEnv, -Env})
-      (Rest <: FUNC{-MI, -CompEnv, -Env, -Adv})
-      (Par <: FUNC{-MI, -CompEnv, -Env, -Adv, -Rest})
+      (Env <: ENV{-MI, -CompGlobs}) (Adv <: ADV{-MI, -CompGlobs, -Env})
+      (Rest <: FUNC{-MI, -CompGlobs, -Env, -Adv})
+      (Par <: FUNC{-MI, -CompGlobs, -Env, -Adv, -Rest})
       (invar_rest : glob Rest -> bool, term_rest : glob Rest -> int,
        invar_par : glob Par -> bool, term_par : glob Par -> int)
       (func' : addr, in_guard_low' : int fset) &m :
@@ -639,11 +679,11 @@ qed.
      disjoint (change_par_adv_pis `|` rest_adv_pis) in_guard' *)
 
 lemma composition
-      (Env <: ENV{-MI, -CompEnv}) (Rest <: FUNC{-MI, -CompEnv, -Env})
-      (Adv1 <: ADV{-MI, -CompEnv, -Env, -Rest})
-      (Par1 <: FUNC{-MI, -CompEnv, -Env, -Rest, -Adv1})
-      (Adv2 <: ADV{-MI, -CompEnv, -Env, -Rest})
-      (Par2 <: FUNC{-MI, -CompEnv, -Env, -Rest, -Adv2})
+      (Env <: ENV{-MI, -CompGlobs}) (Rest <: FUNC{-MI, -CompGlobs, -Env})
+      (Adv1 <: ADV{-MI, -CompGlobs, -Env, -Rest})
+      (Par1 <: FUNC{-MI, -CompGlobs, -Env, -Rest, -Adv1})
+      (Adv2 <: ADV{-MI, -CompGlobs, -Env, -Rest})
+      (Par2 <: FUNC{-MI, -CompGlobs, -Env, -Rest, -Adv2})
       (invar_rest : glob Rest -> bool, term_rest : glob Rest -> int,
        invar_par1 : glob Par1 -> bool, term_par1 : glob Par1 -> int,
        invar_par2 : glob Par2 -> bool, term_par2 : glob Par2 -> int)
@@ -702,3 +742,5 @@ by rewrite
    invar_par2 term_par2
    func' in_guard' &m).
 qed.
+
+end Composition.
